theories/Symbolic/Propositions.v
@@ -1797,7 +1797,7 @@ Module Type SymPropOn
     | eterm_binop   {σ1 σ2 σ3} (op : BinOp σ1 σ2 σ3) (t1 : ETerm σ1) (t2 : ETerm σ2) : ETerm σ3
     | eterm_unop    {σ1 σ2} (op : UnOp σ1 σ2) (t : ETerm σ1) : ETerm σ2
     (* | eterm_tuple   {σs : Ctx Ty} (ts : Env ETerm σs) : ETerm (ty.tuple σs) *)
-    (* | eterm_union   {U : unioni} (K : unionk U) (t : ETerm (unionk_ty U K)) : ETerm (ty.union U) *)
+    | eterm_union   {U : unioni} (K : unionk U) (t : ETerm (unionk_ty U K)) : ETerm (ty.union U)
     (* | eterm_record  (R : recordi) (ts : NamedEnv ETerm (recordf_ty R)) : ETerm (ty.record R) *)
     .
     Global Arguments eterm_relval σ v : clear implicits.
@@ -1857,7 +1857,7 @@ Module Type SymPropOn
         | term_binop op t1 t2         => eterm_binop op (erase t1) (erase t2)
         | term_unop op t              => eterm_unop op (erase t)
         (* | term_tuple ts              => eterm_tuple (env.map (fun _ => erase) ts) *)
-        (* | term_union U K t           => eterm_union K (erase t) *)
+        | term_union U K t           => eterm_union K (erase t)
         (* | term_record R ts           => eterm_record R (env.map (fun _ => erase) ts) *)
         end.
 
@@ -1973,9 +1973,9 @@ Module Type SymPropOn
             uop.evalRel op <$> inst_eterm t0
         (* | @eterm_tuple σs ts => *)
         (*     envrec.of_env (σs := σs) <$> inst_env' ι inst_eterm ts *)
-        (* | @eterm_union U K t0 => *)
-        (*     v <- inst_eterm t0 ;; *)
-        (*     Some (unionv_fold U (existT K v)) *)
+        | @eterm_union U K t0 =>
+            rv <- inst_eterm t0 ;;
+            Some (ty.unionv_fold_rel U (existT K rv))
         (* | @eterm_record R ts => *)
         (*     recordv_fold R <$> inst_namedenv' ι inst_eterm ts *)
         end.
@@ -2116,7 +2116,7 @@ Module Type SymPropOn
       (*   induction IH as [|Δ E σ t _ IHE IHt]; cbn in *. *)
       (*   + reflexivity. *)
       (*   + now rewrite IHt, IHE. *)
-      (* - now rewrite IHt. *)
+      - now rewrite IHt.
       (* - cbn. apply option.map_eq_some. *)
       (*   induction IH as [|Δ E [x σ] t _ IHE IHt]; cbn in *. *)
       (*   + reflexivity. *)
